simplify value-dependent classifications

theories/examples/value_sensitivity_2.v
@@ -28,16 +28,16 @@ Section proof.
 
   (* The invariant guarantees the monotonicity of the declassification. *)
   Definition glinv γ γs :=
-    ((pending γs ∗ classification γ High (1/4))
-   ∨ (shot γs ∗ classification γ Low (1/4)))%I.
+    (∃ α, classification γ α (1/2) ∗
+     ((pending γs ∗ ⌜α = High⌝) ∨ (shot γs ∗ ⌜α = Low⌝)))%I.
 
   Definition N := nroot.@"blabla".
 
   (* We verify that the thread that does the "dumping out" in a loop is secure,
     under the monotonicity assumption. *)
-  Lemma thread1_spec γ γst γs out1 rec1 out2 rec2 ξ :
+  Lemma thread1_spec γ γs out1 rec1 out2 rec2 ξ :
     ⟦ tref (tint Low) ⟧ ξ out1 out2 -∗
-    value_dependent γ γst (tint Low) ξ rec1 rec2 -∗
+    value_dependent γ (tint Low) ξ rec1 rec2 -∗
     inv N (glinv γ γs) -∗
     DWP thread1 out1 rec1 & thread1 out2 rec2 : ⟦ tunit ⟧ ξ.
   Proof.
@@ -45,28 +45,54 @@ Section proof.
     iLöb as "IH". dwp_rec. dwp_pures.
     dwp_bind (is_classified _) (is_classified _).
     iApply (is_classified_spec with "Hvd").
-    iIntros (α) "Ha".
-    iInv N as "[[Htok >Hc]|[#Htok >Hc]]" "Hcl";
-      iDestruct (classification_auth_agree with "Ha Hc") as %->;
-      iFrame "Ha".
-    + iMod ("Hcl" with "[Htok Hc]") as "_".
-      { iNext. iLeft. iFrame. }
-      iModIntro. iSimpl. dwp_pures. iApply "IH".
-    + iMod ("Hcl" with "[Htok Hc]") as "_".
-      { iNext. iRight. by iFrame. }
-      iModIntro. iSimpl. dwp_pures.
-      iApply (logrel_seq with "[-IH] IH").
+    iIntros (α b) "Ha".
+    iInv N as (β) "[>Hc Hi]" "Hcl".
+    iDestruct (classification_auth_agree with "Ha Hc") as %<-.
+    iFrame "Ha". iDestruct "Hi" as ">[[Htok %]|[#Htok %]]"; simplify_eq/=.
+    - iMod ("Hcl" with "[Htok Hc]") as "_".
+      { iNext. iExists _. iFrame. iLeft. eauto with iFrame. }
+      iModIntro. iIntros (Hfoo). assert (b = true) as ->.
+      { destruct b; naive_solver. }
+      iSimpl. dwp_pures. iApply "IH".
+    - iMod ("Hcl" with "[Htok Hc]") as "_".
+      { iNext. iExists _. iFrame. iRight. eauto with iFrame. }
+      iModIntro. iIntros (Hfoo). destruct b.
+      { iSimpl. dwp_pures. iApply "IH". }
+      dwp_pures. iApply (logrel_seq with "[-IH] IH").
       dwp_bind (read_dep _) (read_dep _).
       iApply (read_spec with "Hvd").
       iIntros (α v1 v2) "Ha #Hv".
-      iInv N as "[[>Htok2 >Hc]|[_ >Hc]]" "Hcl".
+      iInv N as (β) "[>Hc Hi]" "Hcl".
+      iDestruct "Hi" as ">[[Htok2 %]|[_ %]]"; simplify_eq/=.
       { iExFalso. iApply (shot_not_pending with "Htok Htok2"). }
       iDestruct (classification_auth_agree with "Ha Hc") as %->.
       iFrame "Ha".
       iMod ("Hcl" with "[Htok Hc]") as "_".
-      { iNext. iRight. by iFrame. }
+      { iNext. iExists _. iFrame. iRight. eauto with iFrame. }
       iModIntro.
       iApply logrel_store; first (by solve_ndisj); iApply dwp_value; eauto with iFrame.
+  Qed.
+
+  Lemma thread2_spec γ γs rec1 rec2 ξ :
+    value_dependent γ (tint Low) ξ rec1 rec2 -∗
+    inv N (glinv γ γs) -∗
+    classification γ High (1/2) -∗
+    DWP thread2 rec1 & thread2 rec2 : ⟦ tunit ⟧ ξ.
+  Proof.
+    iIntros "#Hvd #Hinv Hc2".
+    dwp_rec.
+    iApply (declassify_spec with "Hvd [] Hc2").
+    { rewrite !interp_eq. iExists 0,0. by eauto. }
+    iSimpl. iIntros "Ha Hc2".
+    iInv N as (α') "[>Hc1 >Hi]" "Hcl".
+    iDestruct (classification_auth_agree with "Ha Hc1") as %<-.
+    iCombine "Hc1 Hc2" as "Hc".
+    iMod (classification_update Low with "Ha Hc") as "[$ [Hc1 Hc2]]".
+    iDestruct "Hi" as "[[Htok %]|[Htok %]]"; simplify_eq/=.
+    iMod (shoot with "Htok") as "Htok".
+    iMod ("Hcl" with "[-Hc2]") as "_".
+    { iNext. iExists _. iFrame. eauto with iFrame. }
+    iModIntro. iFrame "Hc2". iIntros "Hc2". eauto.
   Qed.
 
   Lemma proof out1 out2 dat1 dat2 ξ :
@@ -84,40 +110,18 @@ Section proof.
     iApply dwp_alloc. iIntros (is_classified1 is_classified2) "Hc1 Hc2". iNext.
 
     iMod (make_value_dependent (tint Low) with "Hrd1 Hrd2 Hc1 Hc2 []")
-      as (γ γst) "[#Hvd Hc]".
+      as (γ) "[#Hvd Hc]".
     { simpl. rewrite left_id. iExact "Hdat". }
-    iClear "Hdat".
+    iClear "Hdat". iDestruct "Hc" as "[Hc1 Hc2]".
     dwp_pures.
     iMod new_pending as (γs) "Hpend".
 
-    rewrite classification_quarter.
-    iDestruct "Hc" as "[Hc1 Hc]".
+    iMod (inv_alloc N _ (glinv γ γs) with "[-Hc2]") as "#Hinv".
+    { iNext. iExists _. iFrame. iLeft. eauto with iFrame. }
 
-    iMod (inv_alloc N _ (glinv γ γs) with "[-Hc]") as "#Hinv".
-    { iNext. iLeft. by iFrame. }
-
-    iApply (dwp_par (⟦ tunit ⟧ ξ) (⟦ tunit ⟧ ξ) with "[] [Hc]").
+    iApply (dwp_par (⟦ tunit ⟧ ξ) (⟦ tunit ⟧ ξ) with "[] [Hc2]").
     - (* Thread 1 *) iApply (thread1_spec with "Hout Hvd Hinv").
-    - (* Thread 2 *)
-      dwp_rec.
-      iApply (declassify_spec with "Hvd [] Hc").
-      { rewrite !interp_eq. iExists 0,0. by eauto. }
-      iIntros (α) "Ha Hf".
-      assert (Heq : ((3/4)%Qp + (1/4)%Qp)%Qp = 1%Qp).
-      { by apply (bool_decide_unpack _). }
-      iInv N as "[[>Htok >Hc]|[#Htok >Hc]]" "Hcl";
-        iDestruct (classification_auth_agree with "Ha Hc") as %->;
-        iCombine "Hf Hc" as "Hc"; rewrite Heq;
-        iMod (classification_update Low with "Ha Hc") as "[$ Hc]";
-        rewrite classification_quarter;
-        iDestruct "Hc" as "[Hc1 Hc]".
-      + iMod (shoot with "Htok") as "Htok".
-        iMod ("Hcl" with "[Htok Hc1]") as "_".
-        { iNext. iRight. by iFrame. }
-        iModIntro. eauto.
-      + iMod ("Hcl" with "[Htok Hc1]") as "_".
-        { iNext. iRight. by iFrame. }
-        iModIntro. eauto.
+    - (* Thread 2 *) iApply (thread2_spec with "Hvd Hinv Hc2").
     - (* Finally *)
       iIntros (???? [-> ->] [-> ->]).
       iNext. iExists _,_,_,_; eauto with iFrame.
